examples/Imp2Vir/CombinatorsWF.v
@@ -1,7 +1,8 @@
 From Coq Require Import
      Lia
      List
-     NArith.
+     NArith
+     ZArith.
 
 From Vellvm Require Import Syntax.
 
@@ -19,7 +20,7 @@ Definition unique_vector {A} {n} (v : Vector.t A n) : Prop :=
   forall i1 i2, nth v i1 = nth v i2 -> i1 = i2.
 
 Definition unique_bid {ni no} ir : Prop :=
-  forall (vi : Vector.t int ni) (vo : Vector.t int no) vt,
+  forall (vi : Vector.t raw_id ni) (vo : Vector.t raw_id no) vt,
   forall b1 b2,
   unique_vector (vi ++ vt)%vector ->
   List.In b1 (blocks ir vi vo vt) ->
@@ -27,67 +28,371 @@ Definition unique_bid {ni no} ir : Prop :=
   blk_id b1 = blk_id b2 ->
   b1 = b2.
 
-Theorem vector_in_app_iff : forall A n n' (v : Vector.t A n) (v' : Vector.t A n') (a : A),
-  Vector.In a (v ++ v')%vector <-> Vector.In a v \/ Vector.In a v'.
+Theorem nth_firstn : forall A (l : list A) i n a,
+  i < n -> List.nth i (firstn n l) a = List.nth i l a.
 Proof.
-  intros ? ? ? [] [] ?.
-  unfold In in *. simpl in *.
-  apply in_app_iff.
+  induction l ; intros.
+  - rewrite firstn_nil. reflexivity.
+  - induction n.
+    + lia.
+    + rewrite firstn_cons. simpl. induction i.
+      * reflexivity.
+      * rewrite IHl. reflexivity. lia.
 Qed.
 
-Theorem nth_firstn : forall A (l : list A) i n (H : i < n) a,
-  List.nth i l a = List.nth i (firstn n l) a.
+Definition out_blk_id id (b : block typ) : Prop :=
+  match blk_term b with
+  | TERM_Br_1 bid => id = bid
+  | TERM_Br _ bid1 bid2 => id = bid1 \/ id = bid2
+  | _ => False
+  end.
+
+Definition cvir_ids_WF {ni no} ir : Prop :=
+  forall (vi : Vec.t raw_id ni) (vo : Vec.t raw_id no) vt b,
+  (
+    List.In b (blocks ir vi vo vt) ->
+    In (blk_id b) (vi ++ vt)%vector
+  ) /\ (
+    List.In b (blocks ir vi vo vt) ->
+    forall bid,
+    out_blk_id bid b ->
+    In bid (vo ++ vt)%vector
+  ).
+
+Theorem block_cvir_id_WF : forall c, cvir_ids_WF (block_cvir c).
+Proof.
+  unfold cvir_ids_WF.
+  intros ? [] [] [].
+  split ; intros.
+  - simpl in H.
+    destruct H ; [| contradiction ].
+    apply vector_in_app_iff.
+    left.
+    unfold In.
+    subst.
+    simpl.
+    destruct x ; simpl in * ; [lia |].
+    unfold Vec.hd. simpl. intuition.
+  - unfold out_blk_id in H0.
+    simpl in *.
+    destruct H ; [| contradiction ].
+    apply vector_in_app_iff.
+    left.
+    unfold In.
+    subst.
+    simpl in *.
+    subst.
+    destruct x0 ; simpl in * ; [lia |].
+    unfold Vec.hd. simpl. intuition.
+Qed.
+
+Theorem unique_vector_app1 :
+  forall A n1 n2 (v1 : Vec.t A n1) (v2 : Vec.t A n2), unique_vector (v1 ++ v2) -> unique_vector v1.
+Proof.
+  unfold unique_vector.
+  intros.
+  destruct v1, v2, i1, i2.
+  apply unique_fin. simpl.
+  eassert (H1 := H (fi' x1) (fi' x2)).
+  Unshelve.
+  2, 3: simpl; lia.
+  erewrite 2 nth_destruct in H0. simpl in H0.
+  eassert (fi' x1 = fi' x2).
+  apply H1.
+  erewrite 2 nth_destruct. simpl. rewrite 2 app_nth1 ; try lia. exact H0.
+  inversion H2. reflexivity.
+  Unshelve.
+  all: induction x; [simpl in *; lia | auto].
+Qed.
+
+Theorem unique_vector_app2 :
+  forall A n1 n2 (v1 : Vec.t A n1) (v2 : Vec.t A n2), unique_vector (v1 ++ v2) -> unique_vector v2.
+Proof.
+  unfold unique_vector.
+  intros.
+  destruct v1, v2, i1, i2.
+  apply unique_fin. simpl.
+  eassert (H1 := H (fi' (n1 + x1)) (fi' (n1 + x2))).
+  Unshelve.
+  2, 3: simpl; lia.
+  erewrite 2 nth_destruct in H0. simpl in H0.
+  eassert (fi' (n1 + x1) = fi' (n1 + x2)).
+  apply H1.
+  erewrite 2 nth_destruct. simpl. rewrite 2 app_nth2 ; try lia.
+  replace (n1 + x1 - length x) with x1 by lia.
+  replace (n1 + x2 - length x) with x2 by lia.
+  exact H0.
+  inversion H2. lia.
+  Unshelve.
+  all: induction x0; [simpl in *; lia | auto].
+Qed.
+
+Theorem unique_vector_reorder :
+  forall A n1 n2 n3 n4 (v1 : Vec.t A n1) (v2 : Vec.t A n2) (v3 : Vec.t A n3) (v4 : Vec.t A n4), unique_vector ((v1 ++ v2) ++ v3 ++ v4) -> unique_vector ((v1 ++ v3) ++ v2 ++ v4).
+Proof.
+  unfold unique_vector.
+  intros.
+  destruct v1, v2, v3, v4, i1 as [i1 ?], i2 as [i2 ?].
+  erewrite 2 nth_destruct in H0. simpl in H0.
+  apply unique_fin. simpl.
+  set (cast_idx := fun i1 =>
+    if andb (n1 <=? i1) (i1 <? (n1 + n2)) then i1 + n3
+    else if andb ((n1 + n2) <=? i1) (i1 <=? (n1 + n2 + n3)) then i1 - n2
+    else i1
+  ).
+  set (i1' := cast_idx i1).
+  set (i2' := cast_idx i2).
+  subst cast_idx. simpl in i1', i2'.
+  set (bound_idx := fun i1 =>
+    i1 < n1 \/
+    (i1 >= n1 /\ i1 < n1 + n2) \/
+    (i1 >= n1 + n2 /\ i1 < n1 + n2 + n3) \/
+    i1 >= n1 + n2 + n3).
+  assert (H1 : bound_idx i1) by (unfold bound_idx in *; lia).
+  assert (H2 : bound_idx i2) by (unfold bound_idx in *; lia).
+  subst bound_idx. simpl in *.
+  eassert (H' := H (fi' i1') (fi' i2')). destruct H'. subst i1' i2'.
+  rewrite <- 3 Nat.leb_gt in H1, H2.
+  unfold ge in *. rewrite <- 3 Nat.leb_le in H1, H2.
+  intuition.
+  simpl in *. unfold andb. simpl. rewrite * H3. rewrite * H1. simpl.
 Admitted.
+
+Theorem merge_cvir_id_WF :
+  forall ni1 no1 ni2 no2 (ir1 : cvir ni1 no1) (ir2 : cvir ni2 no2),
+  cvir_ids_WF ir1 -> cvir_ids_WF ir2 ->
+  cvir_ids_WF (merge_cvir ir1 ir2).
+Proof.
+  unfold cvir_ids_WF.
+  intros ? ? ? ? ? ? ? ? ? ? ? ?.
+  split_vec vi ni1.
+  split_vec vo no1.
+  split_vec vt (n_int ir1).
+  Opaque Vec.splitat.
+  simpl in *.
+  rewrite 3 splitat_append.
+  edestruct H, H0.
+  rewrite vector_in_app_iff in H1, H3.
+  split ; intros ; rewrite 3 vector_in_app_iff ; apply in_app_iff in H5.
+  - destruct H5 ; apply H1 in H5 + apply H3 in H5 ; destruct H5 ; intuition.
+  - destruct H5 ; eapply H2 in H5 + eapply H4 in H5.
+    2, 4: eassumption.
+    all: rewrite vector_in_app_iff in H5.
+    all: intuition.
+Qed.
+
+Theorem merge_cvir_blocks :
+  forall ni1 no1 ni2 no2 (ir1 : cvir ni1 no1) (ir2 : cvir ni2 no2) vi1 vi2 vo1 vo2 vt1 vt2,
+  blocks (merge_cvir ir1 ir2) (vi1++vi2) (vo1++vo2) (vt1++vt2) = (blocks ir1 vi1 vo1 vt1 ++ blocks ir2 vi2 vo2 vt2)%list.
+Proof.
+  intros.
+  simpl.
+  rewrite 3 splitat_append.
+  reflexivity.
+Qed.
 
 Theorem merge_cvir_unique :
   forall ni1 no1 ni2 no2 (ir1 : cvir ni1 no1) (ir2 : cvir ni2 no2),
-  unique_bid ir1 -> unique_bid ir2 -> unique_bid (merge_cvir ir1 ir2).
+  cvir_ids_WF ir1 ->
+  cvir_ids_WF ir2 ->
+  unique_bid ir1 ->
+  unique_bid ir2 ->
+  unique_bid (merge_cvir ir1 ir2).
 Proof.
   unfold unique_bid.
-  unfold unique_vector.
   intros.
-  apply in_app_iff in H2, H3.
+  split_vec vi ni1.
+  split_vec vo no1.
+  split_vec vt (n_int ir1).
+  rewrite merge_cvir_blocks in H4, H5.
+  rewrite in_app_iff in H4, H5.
+  specialize (H1 vi1 vo1 vt1 b1 b2).
+  specialize (H2 vi2 vo2 vt2 b1 b2).
+  apply unique_vector_reorder in H3.
+  destruct H4, H5.
+  - apply unique_vector_app1 in H3.
+    apply H1.
+    all: assumption.
+  - apply H in H4.
+    apply H0 in H5.
+    eapply In_nth in H4, H5.
+    destruct H4 as [? ?], H5 as [? ?].
+    erewrite <- vector_app_nth1 in H4.
+    erewrite <- vector_app_nth2 in H5.
+    rewrite <- H4 in H6.
+    rewrite <- H5 in H6.
+    specialize (H3 _ _ H6).
+    destruct x, x0.
+    simpl in H3.
+    inversion H3.
+    lia.
+  - apply H0 in H4.
+    apply H in H5.
+    eapply In_nth in H4, H5.
+    destruct H4 as [? ?], H5 as [? ?].
+    erewrite <- vector_app_nth2 in H4.
+    erewrite <- vector_app_nth1 in H5.
+    rewrite <- H4 in H6.
+    rewrite <- H5 in H6.
+    specialize (H3 _ _ H6).
+    destruct x, x0.
+    simpl in H3.
+    inversion H3.
+    lia.
+  - apply unique_vector_app2 in H3.
+    eapply H2.
+    all: assumption.
+Qed.
+(*
+    simpl in H3.
+    replace x0 with (x0 + length (proj1_sig (vi1 ++ vt1)) - length (proj1_sig (vi1 ++ vt1))) in H8 by lia.
+    erewrite <- app_nth2 in H8 ; [| lia].
+
+    eapply List.In_nth in H4, H5.
+    destruct H4, H5.
+    destruct H4, H5.
+    erewrite <- app_nth1 in H7 ; [| assumption].
+    erewrite <- merge_cvir_blocks in H7.
+    replace x0 with (x0 + length (blocks ir1 vi1 vo1 vt1) - length (blocks ir1 vi1 vo1 vt1)) in H8 by lia.
+    erewrite <- app_nth2 in H8 ; [| lia].
+    rewrite <- merge_cvir_blocks in H8.
+    rewrite <- H8 in H6.
+    rewrite <- H7 in H6.
+    simpl in H6.
+
+  unfold unique_vector.
+  intros ? ? ? ? ? ? H8 H9 ? ? ? ? ? ? ? ? ? ? ?.
+  assert (H10 := merge_cvir_id_WF _ _ _ _ ir1 ir2 H8 H9 vi vo vt b1).
+  assert (H10' := merge_cvir_id_WF _ _ _ _ ir1 ir2 H8 H9 vi vo vt b2).
+  split_vec vi ni1.
+  split_vec vo no1.
+  split_vec vt (n_int ir1).
+  specialize (H8 vi1 vo1 vt1). assert (H8' := H8 b2). specialize (H8 b1).
+  specialize (H9 vi2 vo2 vt2). assert (H9' := H9 b2). specialize (H9 b1).
+  destruct H8 as [H8 _], H8' as [H8' _], H9 as [H9 _], H9' as [H9' _], H10 as [H10 _], H10' as [H10' _].
   simpl in *.
+  rewrite vector_in_app_iff in H8, H8', H9, H9'.
+  rewrite 3 splitat_append in H2, H3, H10, H10'.
+  rewrite in_app_iff in H2, H3, H10, H10'.
   destruct H2, H3.
   - eapply H.
     2,3,4: eassumption.
-    intros.
-    destruct vi, vo, vt, i1, i2.
+    intros [] [] ?.
     apply Fin.unique_fin.
-    simpl in *.
-    unfold Vec.append in *.
-    simpl in *.
-    erewrite nth_rewrite in H5.
-    erewrite nth_rewrite in H5.
+    erewrite 2 nth_destruct in H5.
     simpl in H5.
-    assert (x2 < length (firstn ni1 x) \/ x2 >= length (firstn ni1 x)).
-    lia.
-    assert (x3 < length (firstn ni1 x) \/ x3 >= length (firstn ni1 x)).
-    lia.
+    assert (x < length (proj1_sig vi1) \/ x >= length (proj1_sig vi1)) by lia.
+    assert (x0 < length (proj1_sig vi1) \/ x0 >= length (proj1_sig vi1)) by lia.
+    destruct vi1 as [li1 ?], vi2 as [li2 ?], vo1 as [lo1 ?], vo2 as [lo2 ?], vt1 as [lt1 ?], vt2 as [lt2 ?].
+    simpl in *.
     destruct H6, H7.
-    + erewrite 2 app_nth1 in H5 ; try assumption.
-      rewrite firstn_length in H6,H7.
-      epose (x2' := fi' x2). epose (x3' := fi' x3).
-      specialize (H1 x2' x3').
-      erewrite 2 nth_rewrite in H1.
-      simpl in H1.
-      rewrite 2 app_nth1 in H1 ; try lia.
-      rewrite<- 2 nth_firstn in H5 ; try lia.
-      apply H1 in H5.
-      injection H5 as ?.
-      exact H5.
-   + erewrite app_nth1 in H5 ; try assumption.
-     erewrite app_nth2 in H5 ; try assumption.
-     rewrite firstn_length in H5,H6,H7.
-     epose (x2' := fi' x2). epose (x3' := fi' (ni2 + x3)).
-     specialize (H1 x2' x3').
-     erewrite 2 nth_rewrite in H1.
-     simpl in H1.
-     rewrite app_nth1 in H1 ; try lia.
-     rewrite app_nth2 in H1 ; try lia.
-     rewrite<- 2 nth_firstn in H5 ; try lia.
-     rewrite min_l in H5 ; try lia.
-     replace (x3 - ni1) with (ni2 + x3 - length x ) in H5 by lia.
-     apply H1 in H5.
-     injection H5 as ?.
+    all: rewrite app_nth1 in H5 + rewrite app_nth2 in H5 ; [| assumption].
+    all: rewrite app_nth1 in H5 + rewrite app_nth2 in H5 ; [| assumption].
+    all: epose (x' := fi' x) + epose (x' := fi' (ni2 + x));
+      epose (x0' := fi' x0) + epose (x0' := fi' (ni2 + x0));
+      specialize (H1 x' x0');
+      erewrite 2 nth_destruct in H1;
+      simpl in H1;
+      rewrite app_nth1 in H1 + rewrite app_nth2 in H1; [| rewrite app_length ; lia ];
+      rewrite (app_nth1 (_ ++ _)) in H1 + rewrite (app_nth2 (_ ++ _)) in H1; [| rewrite app_length ; lia ].
+    all: try rewrite * app_length in H1.
+    all: rewrite app_nth1 in H1 + rewrite app_nth2 in H1 ; [| lia].
+    all: rewrite app_nth1 in H1 + rewrite app_nth2 in H1 ; [| lia].
+    all: try replace (x - length li1) with (ni2 + x - (length li1 + length li2)) in H5 by lia.
+    all: try replace (x0 - length li1) with (ni2 + x0 - (length li1 + length li2)) in H5 by lia.
+    all: apply H1 in H5.
+    all: injection H5 as ?.
+    all: lia.
+  - intuition.
+    eapply In_nth in H10, H11.
+    destruct H10, H11.
+    rewrite <- H8 in H4.
+    rewrite <- H10 in H4.
+    apply H1 in H4.
+    destruct x, x0.
+    eapply List.In_nth in H2, H3.
+    destruct H2 as [ ? [ ? ? ]], H3 as [ ? [ ? ? ]].
+    inversion H4.
+    subst.
+    apply In_nth in H6, H7.
+    destruct H6, H7.
+Admitted.
+*)
+
+Theorem seq_cvir_id_WF :
+  forall ni1 no1 ni2 no2 (ir1 : cvir ni1 (S no1)) (ir2 : cvir (S ni2) no2),
+  cvir_ids_WF ir1 -> cvir_ids_WF ir2 ->
+  cvir_ids_WF (seq_cvir ir1 ir2).
+Proof.
+  unfold cvir_ids_WF.
+  intros.
+  split_vec vi ni1.
+  split_vec vo no1.
+  simpl in *.
+  destruct (Vec.uncons vt) as [it vt'] eqn:?.
+  apply cons_uncons in Heqp. subst.
+  split_vec vt' (n_int ir1).
+  rewrite 2 splitat_append.
+  edestruct H, H0.
+  split.
+  - intro.
+    apply in_app_iff in H5.
+    rewrite 2 vector_in_app_iff.
+    unfold In. simpl.
+    destruct H5 ; apply H1 in H5 + apply H3 in H5 ; apply in_app_iff in H5 ; simpl in * ; intuition.
+  - intros.
+    rewrite 2 vector_in_app_iff.
+    unfold In. simpl.
+    apply in_app_iff in H5.
+    destruct H5 ; eapply H2 in H5 + eapply H4 in H5; try eassumption ;
+    apply vector_in_app_iff in H5 ; unfold In in H5 ; simpl in H5 ; intuition.
+Qed.
+
+  (*intros.
+  unfold cvir_ids_WF.
+  intros.
+  Opaque merge_cvir.
+  simpl.
+  split.
+  - assert (H1 := merge_cvir_id_WF _ _ _ _ ir1 ir2 H H0).
+    unfold cvir_ids_WF in H1.
+    destruct (Vec.uncons vt) as [it vt'] eqn:?.
+    apply cons_uncons in Heqp. subst.
+    assert (List.In b
+  (blocks
+     (merge_cvir
+        (mk_cvir
+           (fun (vi0 : Vec.t raw_id ni1) (vo0 : Vec.t raw_id no1) (vt0 : Vec.t raw_id (n_int ir1)) =>
+            blocks ir1 vi0 (it :: vo0) vt0))
+        (mk_cvir
+           (fun (vi0 : Vec.t raw_id ni2) (vo0 : Vec.t raw_id no2) (vt0 : Vec.t raw_id (n_int ir2)) =>
+            blocks ir2 (it :: vi0) vo0 vt0))) vi vo vt') -> In (blk_id b) (vi ++ vt')).
+    apply merge_cvir_id_WF.
+    admit. admit.
+    intro.
+    apply Coqlib.list_in_insert.
+    specialize (H2 H3).
+    assumption.*)
+
+Theorem seq_cvir_unique :
+  forall ni1 no1 ni2 no2 (ir1 : cvir ni1 (S no1)) (ir2 : cvir (S ni2) no2),
+  cvir_ids_WF ir1 ->
+  cvir_ids_WF ir2 ->
+  unique_bid ir1 ->
+  unique_bid ir2 ->
+  unique_bid (seq_cvir ir1 ir2).
+Proof.
+  intros.
+  unfold seq_cvir.
+  Opaque merge_cvir.
+  simpl.
+  unfold unique_bid in *.
+  intros.
+  split_vec vi ni1.
+  split_vec vo no1.
+  simpl in *.
+  destruct (Vec.uncons vt) as [it vt'] eqn:?.
+  apply cons_uncons in Heqp. subst.
+  split_vec vt' (n_int ir1).
+  eapply merge_cvir_unique. 6: eassumption. 6: eassumption. all: eauto.
 Admitted.
