examples/Imp2Vir/Vector.v
@@ -29,6 +29,14 @@ Proof.
   reflexivity.
 Qed.
 
+Theorem vector_length : forall A n (v : t A n),
+  length (proj1_sig v) = n.
+Proof.
+  destruct v.
+  simpl.
+  exact e.
+Qed.
+
 Program Definition empty (A : Type) : t A 0 := vec' nil.
 
 Program Definition cons {A} {n} h (v : t A n) : t A (S n) := vec' (h::v).
@@ -77,7 +85,7 @@ Next Obligation.
   - destruct v. simpl in *. subst. discriminate e.
 Qed.
 
-Theorem nth_rewrite : forall A n (v : t A n) i a, nth v i = List.nth (proj1_sig i) (proj1_sig v) a.
+Theorem nth_destruct : forall A n (v : t A n) i a, nth v i = List.nth (proj1_sig i) (proj1_sig v) a.
 Proof.
   intros ? ? [] [] ?.
   subst.
@@ -98,6 +106,61 @@ Defined.
 
 Definition In {A} {n} a (v : t A n) := List.In a (proj1_sig v).
 
+Theorem vector_in_app_iff : forall A n n' (v : Vector.t A n) (v' : Vector.t A n') (a : A),
+  Vector.In a (append v v') <-> Vector.In a v \/ Vector.In a v'.
+Proof.
+  intros ? ? ? [] [] ?.
+  unfold In in *. simpl in *.
+  apply in_app_iff.
+Qed.
+
+Theorem vector_app_nth1 :
+  forall A n n' (v : t A n) (v' : t A n') (k : fin n), nth (append v v') (L n' k) = nth v k.
+Proof.
+  intros.
+  erewrite 2 nth_destruct.
+  destruct v, v', k.
+  simpl in *.
+  rewrite app_nth1; [|lia].
+  apply nth_indep.
+  lia.
+  Unshelve.
+  all: destruct v, k ; destruct x ; [ simpl in e ; lia | assumption ].
+Qed.
+
+Theorem vector_app_nth2 :
+  forall A n n' (v : t A n) (v' : t A n') (k : fin n'), nth (append v v') (R n k) = nth v' k.
+Proof.
+  intros.
+  erewrite 2 nth_destruct.
+  destruct v, v', k.
+  simpl in *.
+  rewrite app_nth2; [| lia].
+  replace (n + x1 - length x) with x1 by lia.
+  apply nth_indep.
+  lia.
+  Unshelve.
+  all: destruct v', k ; destruct x ; [ simpl in e ; lia | assumption ].
+Qed.
+
+Theorem In_nth :
+  forall A n (v : t A n) (x : A), In x v -> exists n : fin n, nth v n = x.
+Proof.
+  intros.
+  unfold In in H.
+  eapply In_nth in H.
+  destruct H as [ n0 [ H H0 ]].
+  eexists (fi' n0).
+  erewrite nth_destruct.
+  simpl.
+  exact H0.
+  Unshelve.
+  2: exact x.
+  simpl.
+  rewrite vector_length in H.
+  exact H.
+Qed.
+
 Program Definition splitat {A} i {j} (v : t A (i+j)) :
   t A i * t A j :=
   (vec' (firstn i (proj1_sig v)), vec' (skipn i (proj1_sig v))).
@@ -109,6 +172,25 @@ Defined.
 Next Obligation.
   destruct v. simpl in *. rewrite skipn_length. apply Nat.add_sub_eq_l. auto.
 Defined.
+
+Theorem splitat_append : forall A n n' (v : t A n) (v' : t A n'),
+  splitat n (append v v') = (v,v').
+Proof.
+  unfold splitat, append.
+  destruct v, v'.
+  simpl.
+  subst.
+  f_equal ; apply vector_proj1_unique ; simpl.
+  - rewrite firstn_app.
+    rewrite firstn_all.
+    rewrite Nat.sub_diag.
+    rewrite app_nil_r.
+    reflexivity.
+  - rewrite skipn_app.
+    rewrite skipn_all.
+    rewrite Nat.sub_diag.
+    reflexivity.
+Qed.
 
 Theorem append_splitat : forall A n n' (v : t A n) (v' : t A n') (v'' : t A (n+n')),
   splitat n v'' = (v, v') -> v'' = append v v'.
@@ -144,6 +226,33 @@ Next Obligation.
   refine (a, vec' l). exact H0.
 Defined.
 
+Theorem uncons_cons : forall A n (v : t A n) a, uncons (cons a v) = (a, v).
+Proof.
+  intros.
+  unfold uncons.
+  simpl.
+  f_equal.
+  apply vector_proj1_unique.
+  simpl.
+  reflexivity.
+Qed.
+
+Theorem cons_uncons : forall A n (v : t A (S n)) (v' : t A n) a, uncons v = (a, v') -> v = cons a v'.
+Proof.
+  intros.
+  destruct v, v'.
+  unfold uncons in H.
+  destruct x.
+  - simpl in e. lia.
+  - simpl in *.
+    unfold cons.
+    simpl.
+    inversion H.
+    subst.
+    apply vector_proj1_unique.
+    reflexivity.
+Qed.
+
 Program Definition rev {A} {n} (v : t A n) : t A n :=
   vec' (rev (proj1_sig v)).
 Next Obligation.
@@ -168,6 +277,17 @@ Next Obligation.
 Defined.
 
 End Vector.
+
+Ltac split_vec v n1 :=
+  let vp := fresh "vp" in
+  let v1 := fresh v "1" in
+  let v2 := fresh v "2" in
+  remember (splitat n1 v) as vp eqn:?Heqvp;
+  destruct vp as [ v1 v2 ] eqn:?Heq;
+  subst vp;
+  symmetry in Heqvp;
+  apply append_splitat in Heqvp;
+  subst v.
 
 Declare Scope vector_scope.
 Delimit Scope vector_scope with vector.
